small transaction

src/Fs7.v
@@ -11,14 +11,16 @@ Definition st_write (s:storage) a v :=
 Definition st_read (s:storage) a :=
   s a.
 
+Definition empty_storage : storage := fun a => 0.
+
 Inductive steppable (A:Type) :=
   | step : (storage -> storage * A) -> steppable A
   | mbind : forall B:Type, steppable B -> (B -> steppable A) -> steppable A
   | mret : A -> steppable A.
-  
+
 Definition read a : steppable nat := step (fun s => (s, st_read s a)).
 Definition write a v : steppable unit := step (fun s => (st_write s a v, tt)).
-  
+
 Notation "'do' x <- y ; z" := (mbind y (fun x => z))
   (left associativity, at level 200, x ident, y at level 100, z at level 200).
 
@@ -31,7 +33,7 @@ Fixpoint run {A:Type} (f:steppable A) (s:storage) (rem:nat) : storage * option (
   | mbind _ a b => match run a s rem with
                    | (s', None) => (s', None)
                    | (s', Some (v, rem')) => run (b v) s' rem'
-                   end         
+                   end
   | mret a => (s, Some (a, rem))
   end.
 
@@ -42,18 +44,43 @@ Ltac find_match n :=
   | [ |- context [ match n with _ => _ end ] ] => idtac
   end.
 
-Ltac case_nat n  :=
-  try (find_match n; destruct n as [|n]; case_nat n).  
+Ltac case_nat n :=
+  try (find_match n; destruct n as [|n]; case_nat n).
 
 Definition normally {R:Type} (f:steppable R) (P:R->Prop) : Prop :=
-  forall s s' n v rem,
-  run f s n = (s', Some (v, rem)) -> P v.
-  
+  forall s' n v rem,
+  run f empty_storage n = (s', Some (v, rem)) -> P v.
+
 Theorem program_ok : normally program (fun v => v = 8).
 Proof.
   unfold normally.
-  intros s s' n v rem.
+  intros s' n v rem.
   unfold run, program.
   simpl.
   case_nat n; crush.
+Qed.
+
+Definition write_two a b :=
+  do _ <- write 0 a;
+  do _ <- write 1 b;
+  do _ <- write 2 1;
+  mret tt.
+
+Definition read_two :=
+  do a <- read 0;
+  do b <- read 1;
+  do c <- read 2;
+  mret (if eq_nat_dec c 1 then Some (a, b) else None).
+
+Theorem pair_ok :
+  forall a b,
+  forall s n r s' n' r' res,
+  run (write_two a b) empty_storage n = (s, r) ->
+  run read_two s n' = (s', Some (res, r')) ->
+  res = None \/ res = Some (a, b).
+Proof.
+  intros a b s n r s' n' r' res.
+  unfold run, read_two, write_two.
+  simpl.
+  case_nat n; case_nat n'; try congruence; crush.
 Qed.
